## 1
### 1 
$$
\begin{gather}
\text{If T is invertible then:} \\
T \circ T^{-1} = ID_{w} \\
\land \\
T^{-1} \circ T = ID_{v} \\
\\
\text{If we apply:} \\
T \circ T^{-1} = ID_{w} \\
(T \circ T^{-1})^{t} = (ID_{w})^{t} \\
(T^{-1})^{t} \circ T^{t} = ID_{w*} \\ \\
T^{-1} \circ T = ID_{v} \\
(T^{-1} \circ T)^{t} = (ID_{v})^{t} \\
T^{t} \circ (T^{-1})^{t} = ID_{v*} \\ \\
\text{Which proves that } T^{t} \text{ is invertible,} \\
\text{and it's inverse is } (T^{-1})^{t}
\end{gather}
$$

### 2
![[Screenshot 2025-10-29 at 7.34.38 AM.png]]